\begin{frame}{Rekursive Darstellung}
    \[\Upsilon(1,k)=1\]
    \[\Upsilon(n,3) = 1\]
    {\small \begin{align*}
        \Upsilon(n,k) 
        =\sum  _{h_1 = \binom{\tau+k-4}{k-2}+\mathrm{max} \left(0;\ n-\binom{\tau+k-3}{\tau-1} - \binom{\tau+k-4}{\tau} \right)}
                ^{\binom{\tau+k-4}{k-2}+\mathrm{min}\left(\binom{\tau+k-4}{\tau-1};\ n-\binom{\tau+k-3}{\tau-1}\right)}
            \left(
                \Upsilon(h_1,k) \cdot \Upsilon(n-h_1,k-1) 
            \right)
    \end{align*}
    }
\end{frame}